Auxilisries added wich needed Equalities and SideEffects, some refactoring

src/updated/src/SubstSemantics.v
@@ -1,109 +1,267 @@
 Require Export Frames.
+Require Export Exceptions.
 
 Import ListNotations.
 
-(*
-Fixpoint match_pattern (p : Pattern) (e : Expression) : Prop :=
-match p with
-| PVar v => match e with
-            | Val (VVar v') => match_pattern p e
-            | _             => False
-            end
-| PLit l => False
-| PCons hd tl => False
-| PTuple l => False
-| PMap l => False
-| PNil => False
+Definition lit_eqb (l1 l2 : Literal) : bool :=
+match l1, l2 with
+ | Atom s, Atom s2 => String.eqb s s2
+ | Integer z , Integer z2  => Z.eqb z z2
+ | _     , _       => false
 end.
-*)
+
+Lemma lit_eqb_eq : forall l1 l2, lit_eqb l1 l2 = true <-> l1 = l2.
+Proof.
+  destruct l1, l2; split; intros; subst; auto; simpl in H; try congruence.
+  * apply eqb_eq in H. now inversion H.
+  * inversion H. subst. simpl. now rewrite eqb_refl.
+  * apply Z.eqb_eq in H. now inversion H.
+  * inversion H. subst. simpl. now rewrite Z.eqb_refl.
+Qed.
+
+Lemma lit_eqb_refl : forall l, lit_eqb l l = true.
+Proof.
+  intro. rewrite lit_eqb_eq. reflexivity.
+Qed.
+
+Fixpoint match_pattern (p : Pattern) (e : ValueExpression) : option (list ValueExpression) :=
+match p with
+| PVar => Some [e]
+(* | PPid x => match e with
+            | EPid p => if Nat.eqb p x then Some [] else None
+            | _      => None
+            end *)
+| PNil => match e with
+          | VNil => Some []
+          | _    => None
+          end
+| PLit l0 => match e with
+             | VLit l => if lit_eqb l l0 then Some [] else None
+             | _      => None
+             end
+| PCons p1 p2 => 
+  match e with
+  | VCons v1 v2 =>
+    match match_pattern p1 v1, match_pattern p2 v2 with
+    | Some l1, Some l2 => Some (l1 ++ l2)
+    | _      , _       => None
+    end
+  | _           => None
+  end
+| PTuple pl => match e with
+              | VTuple vl =>
+                       (fix match_and_bind_elements pl vl :=
+                        match pl with
+                        | [] => 
+                            match vl with
+                            | [] => Some []
+                            | _ => None
+                            end
+                        | p::ps => 
+                            match vl with
+                            | v::vs => 
+                                match (match_pattern p v) with
+                                | Some vl1 => 
+                                    match (match_and_bind_elements ps vs) with
+                                    | Some vl2 => Some (vl1 ++ vl2)
+                                    | _        => None
+                                    end
+                                | _ => None
+                                end
+                            | _ => None
+                            end 
+                        end) pl vl
+              | _ => None
+              end
+| PMap pl => match e with
+              | VMap vl => (fix match_and_bind_elements pl vl :=
+                          match pl with
+                          | [] => 
+                              match vl with
+                              | []  => Some []
+                              | _   => None
+                              end
+                          | (p1,p2)::ps => 
+                              match vl with
+                              | (v1,v2)::vs =>
+                                  match (match_pattern p1 v1), (match_pattern p2 v2) with
+                                  | Some vl1, Some vl1' =>
+                                      match (match_and_bind_elements ps vs) with
+                                      | Some vl2  => Some (vl1 ++ vl1' ++ vl2)
+                                      | _         => None
+                                      end
+                                  | _, _ => None
+                                  end
+                              | _ => None
+                              end
+                          end) pl vl
+              | _  => None
+              end
+end.
+
+Compute (match_pattern (PTuple []) (VTuple []) ).
+Compute (match_pattern (PTuple [PNil]) (VTuple [VNil]) ).
+Compute (match_pattern (PTuple [PNil]) (VTuple [VVar 1]) ).
+Compute (match_pattern (PTuple [PVar]) (VTuple [VNil]) ).
+Compute (match_pattern (PTuple [PVar]) (VTuple [VVar 1]) ).
+Compute (match_pattern (PTuple [PVar; PNil]) (VTuple [VVar 1; VNil]) ).
+Compute (match_pattern (PTuple [PVar; PVar]) (VTuple [VVar 1; VVar 2]) ).
+Compute (match_pattern (PTuple [PVar; PVar]) (VTuple [VVar 1; VNil]) ).
+Compute (match_pattern (PTuple [PVar; PNil]) (VTuple [VVar 1; VVar 2]) ).
+Compute (match_pattern (PTuple [PNil; PVar]) (VTuple [VVar 1; VVar 2]) ).
+Compute (match_pattern (PTuple [PNil; PVar]) (VTuple [VNil; VVar 2]) ).
+
+Compute (match_pattern (PMap [])            (VMap []) ).
+Compute (match_pattern (PMap [(PNil,PNil)]) (VMap [(VNil,VNil)]) ).
+
+Compute (match_pattern (PMap [(PVar,PNil)]) (VMap [(VNil,VNil)]) ).
+Compute (match_pattern (PMap [(PNil,PVar)]) (VMap [(VNil,VNil)]) ).
+Compute (match_pattern (PMap [(PNil,PNil)]) (VMap [(VVar 1,VNil)]) ).
+Compute (match_pattern (PMap [(PNil,PNil)]) (VMap [(VNil,VVar 2)]) ).
+
+Compute (match_pattern (PMap [(PVar,PVar)]) (VMap [(VNil,VNil)]) ).
+Compute (match_pattern (PMap [(PVar,PNil)]) (VMap [(VVar 1,VNil)]) ).
+Compute (match_pattern (PMap [(PVar,PNil)]) (VMap [(VNil,VVar 2)]) ).
+Compute (match_pattern (PMap [(PNil,PVar)]) (VMap [(VVar 1,VNil)]) ).
+Compute (match_pattern (PMap [(PNil,PVar)]) (VMap [(VNil,VVar 2)]) ).
+Compute (match_pattern (PMap [(PNil,PNil)]) (VMap [(VVar 1,VVar 2)]) ).
+
+Compute (match_pattern (PMap [(PVar,PVar)]) (VMap [(VVar 1,VNil)]) ).
+Compute (match_pattern (PMap [(PVar,PVar)]) (VMap [(VNil,VVar 2)]) ).
+Compute (match_pattern (PMap [(PVar,PNil)]) (VMap [(VVar 1,VVar 2)]) ).
+Compute (match_pattern (PMap [(PNil,PVar)]) (VMap [(VVar 1,VVar 2)]) ).
+Compute (match_pattern (PMap [(PVar,PVar)]) (VMap [(VVar 1,VVar 2)]) ).
+
+
+Inductive ProgResult : Type :=
+| Expression (e : Expression) (* RExp *)
+| ValueSequence (vs : list ValueExpression) (* RValSeq *)
+| Exception (e : Exception) (* RExc *)
+.
+
 
 Definition list_subst (l : list ValueExpression) (ξ : Substitution) : Substitution :=
   fold_right (fun v acc => v .: acc) ξ l.
 
 Reserved Notation "⟨ fs , e ⟩ --> ⟨ fs' , e' ⟩" (at level 50).
 
-Inductive step : FrameStack -> Expression -> FrameStack -> Expression -> Prop :=
+Inductive step : FrameStack -> ProgResult -> FrameStack -> ProgResult -> Prop :=
 (**  Reduction rules *)
+
+(** Value Expressions**)
+(**  Cooling *)
+| cool_value v xs:
+  ⟨ xs, Expression (Val v) ⟩ --> ⟨ xs, ValueSequence [v] ⟩
+
 
 (**  Values *)
 (**  Cooling *)
 | cool_Values_empty xs :
-  ⟨ xs, Exp (EValues []) ⟩ --> ⟨ xs, Val (VValues []) ⟩
+  ⟨ xs, Expression (Exp (EValues [])) ⟩ --> ⟨ xs, ValueSequence [] ⟩
 | cool_Values_1 vl e el v xs :
-  ⟨ (FValues vl (e::el))::xs, Val v⟩ --> ⟨ (FValues (vl++[v]) el)::xs, e ⟩
+  ⟨ (FValues vl (e::el))::xs, ValueSequence [v]⟩ --> ⟨ (FValues (vl++[v]) el)::xs, Expression e ⟩
 | cool_Values_2 vl v xs :
-  ⟨ (FValues vl [])::xs, Val v ⟩ --> ⟨ xs, Val (VValues (vl++[v])) ⟩
+  ⟨ (FValues vl [])::xs, ValueSequence [v] ⟩ --> ⟨ xs, ValueSequence (vl++[v]) ⟩
 (**  Heating *)
 | heat_Values e el xs:
-  ⟨ xs, Exp (EValues (e::el)) ⟩ --> ⟨ (FValues [] el)::xs, e ⟩
+  ⟨ xs, Expression (Exp (EValues (e::el))) ⟩ --> ⟨ (FValues [] el)::xs, Expression e ⟩
+
 
 (**  Cons *)
 (**  Cooling *)
 | cool_Cons_1 hd tl xs :
-  ⟨ (FCons1 hd)::xs, Val tl ⟩ --> ⟨ (FCons2 tl)::xs, hd ⟩
+  ⟨ (FCons1 hd)::xs, ValueSequence [tl] ⟩ --> ⟨ (FCons2 tl)::xs, Expression hd ⟩
 | cool_Cons_2 hd tl xs :
-  ⟨ (FCons2 tl)::xs, Val hd ⟩ --> ⟨ xs, Val (VCons hd tl) ⟩
+  ⟨ (FCons2 tl)::xs, ValueSequence [hd] ⟩ --> ⟨ xs, ValueSequence [VCons hd tl] ⟩
 (**  Heating *)
 | heat_Cons hd tl xs :
-  ⟨ xs, Exp (ECons hd tl) ⟩ --> ⟨ (FCons1 hd)::xs, tl ⟩
+  ⟨ xs, Expression (Exp (ECons hd tl)) ⟩ --> ⟨ (FCons1 hd)::xs, Expression tl ⟩
 
 (**  Tuple *)
 (**  Cooling *)
 | cool_Tuple_empty xs :
-  ⟨ xs, Exp (ETuple []) ⟩ --> ⟨ xs, Val (VTuple []) ⟩ (* Is this deterministic? *)
+  ⟨ xs, Expression (Exp (ETuple [])) ⟩ --> ⟨ xs, ValueSequence [ VTuple [] ] ⟩
 | cool_Tuple_1 vl e el v xs :
-  ⟨ (FTuple vl (e::el))::xs, Val v⟩ --> ⟨ (FTuple (vl++[v]) el)::xs, e ⟩
+  ⟨ (FTuple vl (e::el))::xs, ValueSequence [v] ⟩ --> ⟨ (FTuple (vl++[v]) el)::xs, Expression e ⟩
 | cool_Tuple_2 vl v xs :
-  ⟨ (FTuple vl [])::xs, Val v ⟩ --> ⟨ xs, Val (VTuple (vl++[v])) ⟩
+  ⟨ (FTuple vl [])::xs, ValueSequence [v] ⟩ --> ⟨ xs, ValueSequence [ VTuple (vl++[v]) ] ⟩
 (**  Heating *)
 | heat_Tuple e el xs:
-  ⟨ xs, Exp (ETuple (e::el)) ⟩ --> ⟨ (FTuple [] el)::xs, e ⟩
+  ⟨ xs, Expression (Exp (ETuple (e::el))) ⟩ --> ⟨ (FTuple [] el)::xs, Expression e ⟩
+
 
 (**  Map *)
 (**  Cooling *)
 | cool_Map_empty xs :
-  ⟨ xs, Exp (EMap []) ⟩ --> ⟨ xs, Val (VMap []) ⟩
+  ⟨ xs, Expression (Exp (EMap [])) ⟩ --> ⟨ xs, ValueSequence [ VMap [] ] ⟩
 | cool_Map_1  vl sn fs el xs :
-  ⟨ (FMap1 vl sn el)::xs, Val fs ⟩ --> ⟨ (FMap2 vl fs el)::xs, sn ⟩
+  ⟨ (FMap1 vl sn el)::xs, ValueSequence [fs] ⟩ --> ⟨ (FMap2 vl fs el)::xs, Expression sn ⟩
 | cool_Map_2  vl fs sn fs' sn' el xs :
-  ⟨ (FMap2 vl fs ((fs',sn')::el))::xs, Val sn ⟩ --> ⟨ (FMap1 (vl++[(fs,sn)]) sn' el)::xs, fs' ⟩
+  ⟨ (FMap2 vl fs ((fs',sn')::el))::xs, ValueSequence [sn] ⟩ --> ⟨ (FMap1 (vl++[(fs,sn)]) sn' el)::xs, Expression fs' ⟩
 | cool_Map_3  vl fs sn xs :
-  ⟨ (FMap2 vl fs [])::xs, Val sn ⟩ --> ⟨ xs, Val (VMap (vl++[(fs,sn)])) ⟩
+  ⟨ (FMap2 vl fs [])::xs, ValueSequence [sn] ⟩ --> ⟨ xs, ValueSequence [ VMap (vl++[(fs,sn)]) ] ⟩
 (**  Heating *)
 | heat_Map fs sn el xs :
-  ⟨ xs, Exp (EMap ((fs,sn)::el)) ⟩ --> ⟨ (FMap1 [] sn el)::xs, fs ⟩
+  ⟨ xs, Expression (Exp (EMap ((fs,sn)::el))) ⟩ --> ⟨ (FMap1 [] sn el)::xs, Expression fs ⟩
 
-(**  PrimOp *)
+(*
+(**  PrimOp *) (*TODO: Auxiliaries *)
 (**  Cooling *)
-| cool_PrimOp_empty f v xs :
-  ⟨ xs, Exp (EPrimOp f []) ⟩ --> ⟨ xs, Val VNil ⟩ (*TODO: VNil is a placeholder needs f(), but how?*)
-| cool_PrimOp_1  xs :
-  ⟨ (FPrimOp f vl (e::el))::xs, Val v ⟩ --> ⟨ (FPrimOp f (vl++[v]) el)::xs, e ⟩
-| cool_PrimOp_2  xs :
-  ⟨ (FPrimOp f vl [])::xs, Val v ⟩ --> ⟨ xs, Val VNil ⟩ (*TODO: VNil is a placeholder needs f(vl,v), but how?*)
+| cool_PrimOp_empty f xs :
+  ⟨ xs, Expression(Exp (EPrimOp f [])) ⟩ --> ⟨ xs, ValueSequence [VNil] ⟩ (*TODO: VNil is a placeholder needs f(), but how?*)
+| cool_PrimOp_1 f vl e el v xs :
+  ⟨ (FPrimOp f vl (e::el))::xs, ValueSequence [v] ⟩ --> ⟨ (FPrimOp f (vl++[v]) el)::xs, Expression e ⟩
+| cool_PrimOp_2 f vl v xs :
+  ⟨ (FPrimOp f vl [])::xs, ValueSequence [v] ⟩ --> ⟨ xs, ValueSequence [VNil] ⟩ (*TODO: VNil is a placeholder needs f(vl,v), but how?*)
 (**  Heating *)
 | heat_PrimOp f e el xs :
-  ⟨ xs, Exp (EPrimOp f (e::el)) ⟩ --> ⟨ (FPrimOp f [] el)::xs, e ⟩
+  ⟨ xs, Expression (Exp (EPrimOp f (e::el))) ⟩ --> ⟨ (FPrimOp f [] el)::xs, Expression e ⟩
+*)
 
 (**  Let *)
 (**  Cooling *)
-| cool_Let_a l e2 v xs :
-  length vl = l ->
-  ⟨ (FLet l e2)::xs, Val (VValues vl) ⟩ --> ⟨ xs, e2.[ list_subst vl idsubst ] ⟩ (* TODO: e2.[ ? ] *)
-| cool_Let_b e2 v xs :
-  (forall vl, v <> (VValues vl)) ->
-  ⟨ (FLet 1 e2)::xs, Val v ⟩ --> ⟨ xs, e2.[ v /] ⟩
+| cool_Let l e2 vs xs :
+  length vs = l ->
+  ⟨ (FLet l e2)::xs, ValueSequence vs ⟩ --> ⟨ xs, Expression (e2.[ list_subst vs idsubst ]) ⟩ (* TODO: e2.[ ? ] *)
+
 (**  Heating *)
 | heat_Let l e1 e2 xs :
-  ⟨ xs, Exp (ELet l e1 e2) ⟩ --> ⟨ (FLet l e2)::xs, e1 ⟩
+  ⟨ xs, Expression(Exp (ELet l e1 e2)) ⟩ --> ⟨ (FLet l e2)::xs, Expression e1 ⟩
+
 
 (**  Seq *)
 (**  Cooling *)
 | cool_Seq e2 v xs :
-  ⟨ (FSeq e2)::xs, Val v ⟩ --> ⟨ xs, e2 ⟩ (* TODO: e2.[ ? ]*)
+  ⟨ (FSeq e2)::xs, ValueSequence [v] ⟩ --> ⟨ xs, Expression e2 ⟩
 (**  Heating *)
 | heat_Seq e1 e2 xs :
-  ⟨ xs, Exp (ESeq e1 e2) ⟩ --> ⟨ (FSeq e2)::xs, e1 ⟩
+  ⟨ xs, Expression (Exp (ESeq e1 e2)) ⟩ --> ⟨ (FSeq e2)::xs, Expression e1 ⟩
+  
+(**  Fun *)
+(**  Cooling *)
+| cool_fun e vl xs :
+  ⟨ xs, Expression (Exp (EFun vl e)) ⟩ --> ⟨ xs, ValueSequence [ VClos [] 0 vl e ] ⟩ (*TODO : id not 0*)
+
+
+(**  Call *) (*TODO : will be the same as PrimOp, use the eval from the Auxilieries*)
+(**  Cooling *)
+(**  Heating *)
+
+(**  App *) (* On paper *)
+(**  Cooling *)
+(**  Heating *)
+
+(**  Case *) (*ok*)
+(**  Cooling *)
+(**  Heating *)
+
+(**  LetRec *)
+(**  Cooling *)
+(**  Heating *)
+
+(**  Try *)
+(**  Cooling *)
+(**  Heating *)
 
 where "⟨ fs , e ⟩ --> ⟨ fs' , e' ⟩" := (step fs e fs' e').
 
