src/updated/src/Auxiliaries.v
@@ -1,0 +1,992 @@
+(* Require Core_Erlang_Side_Effects. *) (* TODO: Not implemented*)
+Require Coq.Sorting.Permutation.
+
+Require Export Frames.
+Require Export Exceptions.
+Require Export SideEffects.
+Require Export Equalities.
+
+Module Auxiliaries.
+
+(* Export Core_Erlang_Side_Effects.Side_Effects. *) (* TODO: Not implemented*)
+Export SideEffects.Side_Effects.
+Export Coq.Sorting.Permutation.
+
+Import ListNotations.
+Import Equalities.
+
+(**
+  Built-in function simulation
+
+  BIFCode: we need it in order to enable better pattern-matching on strings
+ *)
+
+Inductive BIFCode :=
+| BPlus | BMinus | BMult | BDivide | BRem | BDiv | BSl | BSr | BAbs
+| BFwrite | BFread 
+| BAnd | BOr | BNot
+| BEq | BTypeEq | BNeq | BTypeNeq
+| BApp | BMinusMinus
+| BTupleToList | BListToTuple
+| BLt | BLe | BGt | BGe
+| BLength | BTupleSize
+| BTl | BHd
+| BElement | BSetElement
+| BIsNumber | BIsInteger | BIsAtom | BIsBoolean
+| BError
+| PMatchFail
+| BNothing
+.
+
+Definition convert_string_to_code (s : string) : BIFCode :=
+match s with
+| "+"%string => BPlus
+| "-"%string => BMinus
+| "*"%string => BMult
+| "/"%string => BDivide
+| "bsl"%string => BSl
+| "bsr"%string => BSr
+| "rem"%string => BRem
+| "div"%string => BDiv
+| "abs"%string => BAbs
+| "fwrite"%string => BFwrite
+| "fread"%string => BFread
+| "and"%string => BAnd
+| "or"%string => BOr
+| "not"%string => BNot
+| "=="%string => BEq
+| "=:="%string => BTypeEq
+| "/="%string => BNeq
+| "=/="%string => BTypeNeq
+| "++"%string => BApp
+| "--"%string => BMinusMinus
+| "tuple_to_list"%string => BTupleToList
+| "list_to_tuple"%string => BListToTuple
+| "<"%string => BLt
+| ">"%string => BGt
+| "=<"%string => BLe
+| ">="%string => BGe
+| "length"%string => BLength
+| "tuple_size"%string => BTupleSize
+| "hd"%string => BHd
+| "tl"%string => BTl
+| "element"%string => BElement
+| "setelement"%string => BSetElement
+| "is_number"%string => BIsNumber
+| "is_integer"%string => BIsInteger
+| "is_atom"%string => BIsAtom
+| "is_boolean"%string => BIsBoolean
+| "error"%string => BError
+(** primops *)
+| "match_fail"%string => PMatchFail
+(** anything else *)
+| _ => BNothing
+end.
+
+(** Semantic domain *)
+Definition ValueSequence := list ValueExpression.
+
+(** For biuilt-in arithmetic calls *)
+Definition eval_arith (fname : string) (params : list ValueExpression) :  ValueSequence + Exception :=
+match convert_string_to_code fname, params with
+(** addition *)
+| BPlus, [VLit (Integer a); VLit (Integer b)] => inl [VLit (Integer (a + b))]
+| BPlus, [a; b]                               => inr (badarith (VTuple [VLit (Atom fname); a; b]))
+(** subtraction *)
+| BMinus, [VLit (Integer a); VLit (Integer b)] => inl [VLit (Integer (a - b))]
+| BMinus, [a; b]                               => inr (badarith (VTuple [VLit (Atom fname); a; b]))
+(** unary minus *)
+| BMinus, [VLit (Integer a)]                   => inl [VLit (Integer (0 - a))]
+| BMinus, [a]                                  => inr (badarith (VTuple [VLit (Atom fname); a]))
+(** unary plus *)
+| BPlus, [VLit (Integer a)]                   => inl [VLit (Integer a)]
+| BPlus, [a]                                  => inr (badarith (VTuple [VLit (Atom fname); a]))
+(** multiplication *)
+| BMult, [VLit (Integer a); VLit (Integer b)] => inl [VLit (Integer (a * b))]
+| BMult, [a; b]                               => inr (badarith (VTuple [VLit (Atom fname); a; b]))
+(** division *)
+| BDivide, [VLit (Integer a); VLit (Integer 0)] => inr (badarith (VTuple [VLit (Atom fname); VLit (Integer a); VLit (Integer 0)]))
+| BDivide, [VLit (Integer a); VLit (Integer b)] => inl [VLit (Integer (a / b))]
+| BDivide, [a; b]                               => inr (badarith (VTuple [VLit (Atom fname); a; b]))
+(** rem *)
+| BRem, [VLit (Integer a); VLit (Integer 0)] => inr (badarith (VTuple [VLit (Atom fname); VLit (Integer a); VLit (Integer 0)]))
+| BRem, [VLit (Integer a); VLit (Integer b)] => inl [VLit (Integer (Z.rem a b))]
+| BRem, [a; b]                               => inr (badarith (VTuple [VLit (Atom fname); a; b]))
+(** div *)
+| BDiv, [VLit (Integer a); VLit (Integer 0)] => inr (badarith (VTuple [VLit (Atom fname); VLit (Integer a); VLit (Integer 0)]))
+| BDiv, [VLit (Integer a); VLit (Integer b)] => inl [VLit (Integer (Z.quot a b))]
+| BDiv, [a; b]                               => inr (badarith (VTuple [VLit (Atom fname); a; b]))
+(** bsl *)
+| BSl, [VLit (Integer a); VLit (Integer b)]  => inl [VLit (Integer (Z.shiftl a b))]
+| BSl, [a; b]                                => inr (badarith (VTuple [VLit (Atom fname); a; b]))
+(** bsr *)
+| BSr, [VLit (Integer a); VLit (Integer b)]  => inl [VLit (Integer (Z.shiftr a b))]
+| BSr, [a; b]                                => inr (badarith (VTuple [VLit (Atom fname); a; b]))
+(** abs *)
+| BAbs, [VLit (Integer a)]                   => inl [VLit (Integer (Z.abs a))]
+| BAbs, [a]                                  => inr (badarg (VTuple [VLit (Atom fname); a]))
+(** anything else *)
+| _         , _                              => inr (undef (VLit (Atom fname)))
+end.
+
+(* TODO: ? *)
+
+(** For IO maniputaion: *)
+Definition eval_io (fname : string) (params : list ValueExpression) (eff : SideEffectList) 
+   : ((ValueSequence + Exception) * SideEffectList) :=
+match convert_string_to_code fname, length params, params with
+(** writing *)
+| BFwrite, 1, _ => (inl [ok]                                  , eff ++ [(Output, params)])
+(** reading *)
+| BFread, 2, e => (inl [VTuple [ok; nth 1 params ErrorValue]], eff ++ [(Input, params)])
+(** anything else *)
+| _              , _, _ => (inr (undef (VLit (Atom fname)))           , eff)
+end.
+
+
+Definition eval_logical (fname : string) (params : list ValueExpression) : ValueSequence + Exception :=
+match convert_string_to_code fname, params with
+(** logical and *)
+| BAnd, [a; b] => 
+   match a, b with
+   | VLit (Atom "true") , VLit (Atom "true")    => inl [ttrue]
+   | VLit (Atom "false"), VLit (Atom "true")    => inl [ffalse]
+   | VLit (Atom "true") , VLit (Atom "false")   => inl [ffalse]
+   | VLit (Atom "false"), VLit (Atom "false")   => inl [ffalse]
+   | _                         , _              => inr (badarg (VTuple [VLit (Atom fname); a; b]))
+   end
+(** logical or *)
+| BOr, [a; b] =>
+   match a, b with
+   | VLit (Atom "true") , VLit (Atom "true")    => inl [ttrue]
+   | VLit (Atom "false"), VLit (Atom "true")    => inl [ttrue]
+   | VLit (Atom "true") , VLit (Atom "false")   => inl [ttrue]
+   | VLit (Atom "false"), VLit (Atom "false")   => inl [ffalse]
+   | _                         , _              => inr (badarg (VTuple [VLit (Atom fname); a; b]))
+   end
+(** logical not *)
+| BNot, [a] =>
+   match a with
+   | VLit (Atom "true")  => inl [ffalse]
+   | VLit (Atom "false") => inl [ttrue]
+   | _                   => inr (badarg (VTuple [VLit (Atom fname); a]))
+   end
+(** anything else *)
+| _ , _ => inr (undef (VLit (Atom fname)))
+end.
+
+(* TODO: ? *)
+
+Definition eval_equality (fname : string) (params : list ValueExpression) : ValueSequence + Exception :=
+match convert_string_to_code fname, params with
+| BEq,  [v1; v2] (* TODO: with floats, this one should be adjusted *)
+| BTypeEq, [v1; v2] => if Value_eqb v1 v2 then inl [ttrue] else inl [ffalse]
+| BNeq,  [v1; v2] (* TODO: with floats, this one should be adjusted *)
+| BTypeNeq, [v1; v2] => if Value_eqb v1 v2 then inl [ffalse] else inl [ttrue]
+(** anything else *)
+| _ , _ => inr (undef (VLit (Atom fname)))
+end.
+
+
+Fixpoint is_shallow_proper_list (v : ValueExpression) : bool :=
+match v with
+| VNil => true
+| VCons x y => is_shallow_proper_list y
+| _ => false
+end.
+
+Fixpoint eval_append (v1 v2 : ValueExpression) : ValueSequence + Exception :=
+match v1, v2 with
+| VNil, x => inl [x]
+| VCons x y, x' => match eval_append y x' with
+                   | inr ex    => inr (badarg (VTuple [VLit (Atom "++"); v1; v2]))
+                   | inl [res] => inl [VCons x res]
+                   | _ => inr (badarg (VTuple [VLit (Atom "++"); v1; v2]))
+                   end
+| _, _ => inr (badarg (VTuple [VLit (Atom "++"); v1; v2]))
+end.
+
+(* TODO: ? *)
+
+Fixpoint subtract_elem (v1 v2 : ValueExpression) : ValueExpression :=
+match v1 with
+| VNil => VNil
+| VCons x y =>
+  match y with
+  | VNil => if Value_eqb x v2 then VNil else VCons x y
+  | VCons z w => if Value_eqb x v2 then y else VCons x (subtract_elem y v2)
+  | z => if Value_eqb x v2 then VCons z VNil else if Value_eqb z v2 then VCons x VNil else VCons x y
+  end
+| _ => ErrorValue
+end.
+
+
+(* TODO: ? *)
+Fixpoint eval_subtract (v1 v2 : ValueExpression) : ValueSequence + Exception :=
+if andb (is_shallow_proper_list v1) (is_shallow_proper_list v2) then
+  match v1, v2 with
+  | VNil, VNil => inl [VNil]
+  | VNil, VCons x y => inl [VNil]
+  | VCons x y, VNil => inl [VCons x y]
+  | VCons x y, VCons x' y' => 
+     match y' with
+     | VNil => inl [subtract_elem (VCons x y) x']
+     | VCons z w => eval_subtract (subtract_elem (VCons x y) x') y'
+     | z => inl [subtract_elem (subtract_elem (VCons x y) x') z]
+     end
+  | _        , _         => inr (badarg (VTuple [VLit (Atom "--"); v1; v2]))
+  end
+else
+  inr (badarg (VTuple [VLit (Atom "--"); v1; v2])).
+
+(* TODO: ? *)
+Definition eval_transform_list (fname : string) (params : list ValueExpression) : ValueSequence + Exception :=
+match convert_string_to_code fname, params with
+| BApp, [v1; v2]        => eval_append v1 v2
+| BMinusMinus, [v1; v2] => eval_subtract v1 v2
+| _ , _ => inr (undef (VLit (Atom fname)))
+end.
+
+Definition transform_tuple (v : ValueExpression) : ValueSequence + Exception :=
+match v with
+| VTuple l => inl [((fix unfold_list l :=
+                   match l with
+                   | [] => VNil
+                   | x::xs => VCons x (unfold_list xs)
+                   end) l)]
+| _        => inr (badarg (VTuple [VLit (Atom "tuple_to_list"); v]))
+end.
+
+Fixpoint transform_list (v : ValueExpression) : list ValueExpression + Exception :=
+match v with
+| VNil      => inl []
+| VCons x y => match y with
+               | VNil => inl [x]
+               | VCons z w => match (transform_list y) with
+                              | inr ex => inr ex
+                              | inl res => inl (x::res)
+                              end
+               | _ => inr (badarg (VTuple [VLit (Atom "list_to_tuple"); v]))
+               end
+| _         => inr (badarg (VTuple [VLit (Atom "list_to_tuple"); v]))
+end.
+
+Definition eval_list_tuple (fname : string) (params : list ValueExpression) : ValueSequence + Exception :=
+match convert_string_to_code fname, params with
+| BTupleToList, [v] => transform_tuple v
+| BListToTuple, [v] => match (transform_list v) with
+                                 | inr ex => inr ex
+                                 | inl l => inl [VTuple l]
+                                 end
+| _                     , _   => inr (undef (VLit (Atom fname)))
+end.
+
+(* TODO: ? *)
+Definition eval_cmp (fname : string) (params : list ValueExpression) : ValueSequence + Exception :=
+match convert_string_to_code fname, params with
+| BLt,  [v1; v2] => if Value_ltb v1 v2 then inl [ttrue] else inl [ffalse]
+| BLe, [v1; v2] => if orb (Value_ltb v1 v2) (Value_eqb v1 v2) 
+                           then inl [ttrue] else inl [ffalse]
+| BGt,  [v1; v2] => if Value_ltb v2 v1 then inl [ttrue] else inl [ffalse]
+| BGe, [v1; v2] => if orb (Value_ltb v2 v1) (Value_eqb v1 v2) 
+                           then inl [ttrue] else inl [ffalse]
+(** anything else *)
+| _ , _ => inr (undef (VLit (Atom fname)))
+end.
+
+
+Definition eval_length (params : list ValueExpression) : ValueSequence + Exception :=
+match params with
+| [v] => let res :=
+          (fix len val := match val with
+                         | VNil => inl Z.zero
+                         | VCons x y => let res := len y in
+                                          match res with
+                                          | inl n => inl (Z.add 1 n)
+                                          | inr _ => res
+                                          end
+                         | _ => inr (badarg (VTuple [VLit (Atom "length"); v]))
+                         end) v in
+        match res with
+        | inl n => inl [VLit (Integer n)]
+        | inr ex => inr ex
+        end
+| _ => inr (undef (VLit (Atom "length")))
+end.
+
+Definition eval_tuple_size (params : list ValueExpression) : ValueSequence + Exception :=
+match params with
+| [VTuple l] => inl [VLit (Integer (Z.of_nat (length l)))]
+| [v] => inr (badarg (VTuple [VLit (Atom "tuple_size"); v]))
+| _ => inr (undef (VLit (Atom "tuple_size")))
+end.
+
+Definition eval_hd_tl (fname : string) (params : list ValueExpression) : ValueSequence + Exception :=
+match convert_string_to_code fname, params with
+| BHd, [VCons x y] => inl [x]
+| BHd, [v] => inr (badarg (VTuple [VLit (Atom fname); v]))
+| BTl, [VCons x y] => inl [y]
+| BTl, [v] => inr (badarg (VTuple [VLit (Atom fname); v]))
+| _, _ => inr (undef (VLit (Atom fname)))
+end.
+
+Fixpoint replace_nth_error {A : Type} (l : list A) (i : nat) (e : A) : option (list A) :=
+match i, l with
+| 0, x::xs => Some (e::xs)
+| _, [] => None
+| S n, x::xs => match (replace_nth_error xs n e) with
+               | None => None
+               | Some l' => Some (x::l')
+               end
+end.
+
+Definition eval_elem_tuple (fname : string) (params : list ValueExpression) : ValueSequence + Exception :=
+match convert_string_to_code fname, params with
+| BElement, [VLit (Integer i); VTuple l] =>
+    match i with
+    | Z.pos p => match nth_error l (pred (Pos.to_nat p)) with
+                 | None   => inr (badarg (VTuple [VLit (Atom fname); VLit (Integer i); VTuple l]))
+                 | Some v => inl [v]
+                 end
+    | _       => inr (badarg (VTuple [VLit (Atom fname); VLit (Integer i); VTuple l]))
+    end
+| BElement, [v1; v2] => inr (badarg (VTuple [VLit (Atom fname); v1; v2]))
+| BSetElement, [VLit (Integer i); VTuple l; val] =>
+    match i with
+    | Z.pos p => match replace_nth_error l (pred (Pos.to_nat p)) val with
+                 | None    => inr (badarg (VTuple [VLit (Atom fname); VLit (Integer i); VTuple l; val]))
+                 | Some l' => inl [VTuple l']
+                 end
+    | _       => inr (badarg (VTuple [VLit (Atom fname); VLit (Integer i); VTuple l]))
+    end
+| BSetElement, [v1; v2; v3] => inr (badarg (VTuple [VLit (Atom fname); v1; v2; v3]))
+| _, _ => inr (undef (VLit (Atom fname)))
+end.
+
+Definition eval_check (fname : string) (params : list ValueExpression) : ValueSequence + Exception := 
+match convert_string_to_code fname, params with
+| BIsNumber, [VLit (Integer i)]     => inl [ttrue]
+| BIsNumber, [_]                    => inl [ffalse]
+| BIsInteger, [VLit (Integer i)]    => inl [ttrue]
+| BIsInteger, [_]                   => inl [ffalse] 
+| BIsAtom, [VLit (Atom a)]          => inl [ttrue]
+| BIsAtom, [_]                      => inl [ffalse]
+| BIsBoolean, [VLit (Atom "true")]
+| BIsBoolean, [VLit (Atom "false")] => inl [ttrue]
+| BIsBoolean, [_]                   => inl [ffalse]
+| _, _              => inr (undef (VLit (Atom fname)))
+end.
+
+Definition eval_error (fname : string) (params : list ValueExpression) : Exception :=
+match params with
+| [VTuple [val]] => (Error, val, VNil)
+| [VTuple [val; reas]] => (Error, val, reas)
+| [val]        => (Error, val, VNil)
+| [val1; val2] => (Error, val1, val2)
+| _            => undef (VLit (Atom fname))
+end.
+
+
+(* TODO: Always can be extended, this function simulates inter-module calls *)
+Definition eval (fname : string) (params : list ValueExpression) (eff : SideEffectList) 
+   : ((ValueSequence + Exception) * SideEffectList) :=
+match convert_string_to_code fname with
+| BPlus | BMinus | BMult | BDivide | BRem | BDiv
+| BSl   | BSr    | BAbs                           => (eval_arith fname params, eff)
+| BFwrite | BFread                                => eval_io fname params eff
+| BAnd | BOr | BNot                               => (eval_logical fname params, eff)
+| BEq | BTypeEq | BNeq | BTypeNeq                 => (eval_equality fname params, eff)
+| BApp | BMinusMinus                              => (eval_transform_list fname params, eff)
+| BTupleToList | BListToTuple                     => (eval_list_tuple fname params, eff)
+| BLt | BGt | BLe | BGe                           => (eval_cmp fname params, eff)
+| BLength                                         => (eval_length params, eff)
+| BTupleSize                                      => (eval_tuple_size params, eff)
+| BHd | BTl                                       => (eval_hd_tl fname params, eff)
+| BElement | BSetElement                          => (eval_elem_tuple fname params, eff)
+| BIsNumber | BIsInteger | BIsAtom | BIsBoolean   => (eval_check fname params, eff)
+| BError | PMatchFail                             => (inr (eval_error fname params), eff)
+(** anything else *)
+| BNothing                                        => (inr (undef (VLit (Atom fname))), eff)
+end.
+
+
+Theorem eval_effect_extension fname vals eff1 res eff2 :
+  eval fname vals eff1 = (res, eff2)
+->
+  exists l', eff2 = eff1 ++ l'.
+Proof.
+  intros. unfold eval in H.
+  destruct (convert_string_to_code fname) eqn:Hfname; simpl in H.
+  all: try (unfold eval_arith, eval_logical, eval_equality,
+             eval_transform_list, eval_list_tuple, eval_cmp,
+             eval_hd_tl, eval_elem_tuple, eval_check, eval_error in H; rewrite Hfname in H; destruct vals;
+    [ inversion H; exists []; rewrite app_nil_r; auto |
+      destruct v; try (destruct vals; inversion H; exists []; rewrite app_nil_r; auto) ]).
+  * unfold eval_io in H; rewrite Hfname in H; destruct (length vals) eqn:Hl; inversion H.
+    - exists []; rewrite app_nil_r. auto.
+    - destruct n.
+      + inversion H. exists [(Output, vals)]. auto.
+      + inversion H. exists []; rewrite app_nil_r. auto.
+  * unfold eval_io in H; rewrite Hfname in H; destruct (length vals) eqn:Hl; inversion H.
+    - exists []; rewrite app_nil_r. auto.
+    - destruct n.
+      + inversion H. exists []; rewrite app_nil_r. auto.
+      + destruct n.
+        ** inversion H.  exists [(Input, vals)]. auto.
+        ** inversion H. exists []; rewrite app_nil_r. auto.
+  * unfold eval_length in H.
+    destruct vals; inversion H; exists []; rewrite app_nil_r; auto.
+  * unfold eval_tuple_size in H.
+    destruct vals; inversion H; exists []; rewrite app_nil_r; auto.
+  * inversion H. exists []; rewrite app_nil_r; auto.
+  * inversion H. exists []; rewrite app_nil_r; auto.
+  * inversion H. exists []; rewrite app_nil_r; auto.
+Qed.
+
+Theorem eval_effect_exists_snd {fname vals eff} :
+  exists eff', snd (eval fname vals eff) = eff'.
+Proof.
+  unfold eval. destruct (convert_string_to_code fname) eqn:Hfname.
+  all: try ( unfold eval_arith, eval_logical, eval_equality,
+             eval_transform_list, eval_list_tuple, eval_cmp,
+             eval_hd_tl, eval_elem_tuple, eval_check, eval_error; rewrite Hfname; destruct vals; 
+             [ exists eff | simpl; auto ]).
+  all: simpl; auto.
+  1-9, 12-39: exists eff; auto.
+  * unfold eval_io. rewrite Hfname. destruct (length vals).
+    - exists eff. auto.
+    - destruct n. eexists. simpl. reflexivity.
+      eexists. reflexivity.
+  * unfold eval_io. rewrite Hfname. destruct (length vals).
+    - exists eff. auto.
+    - destruct n. eexists. simpl. reflexivity.
+      eexists. reflexivity.
+Qed.
+
+Theorem eval_effect_irrelevant_snd {fname vals eff eff'}:
+  snd (eval fname vals eff) = eff ++ eff'
+->
+  forall eff0, snd (eval fname vals eff0) = eff0 ++ eff'.
+Proof.
+  intros.
+  unfold eval in *. destruct (convert_string_to_code fname) eqn:Hfname.
+  all: try (unfold eval_arith, eval_logical, eval_equality,
+             eval_transform_list, eval_list_tuple, eval_cmp,
+             eval_hd_tl, eval_elem_tuple, eval_check in *; rewrite Hfname in *; destruct vals;
+    simpl in *; rewrite <- app_nil_r in H at 1; apply app_inv_head in H; subst;
+             rewrite app_nil_r; reflexivity).
+  * unfold eval_io in *. rewrite Hfname in *. destruct (length vals).
+    - simpl in *; rewrite <- app_nil_r in H at 1; apply app_inv_head in H; subst;
+             rewrite app_nil_r; reflexivity.
+    - destruct n; simpl in *.
+      + apply app_inv_head in H. rewrite H. reflexivity.
+      + rewrite <- app_nil_r in H at 1; apply app_inv_head in H; subst;
+             rewrite app_nil_r; reflexivity.
+  * unfold eval_io in *. rewrite Hfname in *. destruct (length vals).
+    - simpl in *; rewrite <- app_nil_r in H at 1; apply app_inv_head in H; subst;
+             rewrite app_nil_r; reflexivity.
+    - destruct n; simpl in *.
+      + simpl in *; rewrite <- app_nil_r in H at 1; apply app_inv_head in H; subst;
+             rewrite app_nil_r; reflexivity.
+      + destruct n.
+        ** apply app_inv_head in H. rewrite H. reflexivity.
+        ** rewrite <- app_nil_r in H at 1; apply app_inv_head in H; subst;
+             rewrite app_nil_r; reflexivity.
+  * unfold eval_length. simpl in *.
+    rewrite <- app_nil_r in H at 1; apply app_inv_head in H; subst;
+             rewrite app_nil_r; reflexivity.
+  * unfold eval_tuple_size in *.
+    rewrite <- app_nil_r in H at 1; apply app_inv_head in H; subst;
+             rewrite app_nil_r; reflexivity.
+  * rewrite <- app_nil_r in H at 1; apply app_inv_head in H; subst;
+             rewrite app_nil_r; reflexivity.
+  * rewrite <- app_nil_r in H at 1; apply app_inv_head in H; subst;
+             rewrite app_nil_r; reflexivity.
+  * rewrite <- app_nil_r in H at 1; apply app_inv_head in H; subst;
+             rewrite app_nil_r; reflexivity.
+Qed.
+
+Theorem eval_effect_irrelevant_fst {fname vals eff eff0}:
+  fst (eval fname vals eff) = fst (eval fname vals eff0).
+Proof.
+  unfold eval. destruct (convert_string_to_code fname) eqn:Hfname.
+  all: try (unfold eval_arith, eval_logical, eval_equality,
+             eval_transform_list, eval_list_tuple, eval_cmp,
+             eval_hd_tl, eval_elem_tuple, eval_check; rewrite Hfname; destruct vals;
+    [ reflexivity |
+      destruct v; try (destruct vals; auto) ]).
+  * unfold eval_io. rewrite Hfname. destruct (length vals).
+    - reflexivity.
+    - destruct n; reflexivity.
+  * unfold eval_io. rewrite Hfname. destruct (length vals).
+    - reflexivity.
+    - destruct n. reflexivity.
+      + destruct n; reflexivity.
+  * unfold eval_length. reflexivity.
+  * reflexivity.
+  * reflexivity.
+  * reflexivity.
+  * reflexivity.
+Qed.
+
+Theorem eval_effect_extension_snd fname vals eff1 eff2 :
+  snd (eval fname vals eff1) = eff2
+->
+  exists l', eff2 = eff1 ++ l'.
+Proof.
+  intros.
+  pose (eval_effect_extension fname vals eff1 (fst (eval fname vals eff1)) eff2).
+  assert (eval fname vals eff1 = (fst (eval fname vals eff1), eff2)).
+  {
+    rewrite surjective_pairing at 1.
+    rewrite H. auto.
+  }
+  apply e. assumption.
+Qed.
+
+Theorem eval_effect_permutation f vals eff eff' :
+  Permutation eff eff'
+->
+  Permutation (snd (eval f vals eff)) (snd (eval f vals eff')).
+Proof.
+  intros.
+  unfold eval. destruct (convert_string_to_code f) eqn:Hfname.
+  all: try (unfold eval_arith, eval_logical, eval_equality,
+             eval_transform_list, eval_list_tuple, eval_cmp,
+             eval_hd_tl, eval_elem_tuple, eval_check; rewrite Hfname; destruct vals; auto).
+  * unfold eval_io. rewrite Hfname. destruct (length vals).
+    - simpl. auto.
+    - destruct n.
+      + simpl. apply Permutation_app_tail. auto.
+      + auto.
+  * unfold eval_io. rewrite Hfname. destruct (length vals).
+    - auto.
+    - destruct n. auto.
+      destruct n.
+      + simpl. apply Permutation_app_tail. auto.
+      + auto.
+  * unfold eval_length. auto.
+  * auto.
+  * auto.
+  * auto.
+  * auto.
+Qed.
+
+Proposition plus_comm_basic {e1 e2 t : ValueExpression} {eff : SideEffectList} : 
+eval "+"%string [e1 ; e2] eff = (inl [t], eff)
+->
+eval "+"%string [e2; e1] eff = (inl [t], eff).
+Proof.
+  simpl. case_eq e1; case_eq e2; intros.
+  all: try(reflexivity || inversion H1).
+  all: try(destruct l); try(destruct l0); try(reflexivity || inversion H1).
+  * unfold eval, eval_arith. simpl. rewrite <- Z.add_comm. reflexivity.
+Qed.
+
+Proposition plus_comm_basic_value {e1 e2 v : ValueExpression} (eff eff2 : SideEffectList) : 
+  eval "+"%string [e1 ; e2] eff = (inl [v], eff)
+->
+  eval "+"%string [e2; e1] eff2 = (inl [v], eff2).
+Proof.
+  simpl. case_eq e1; case_eq e2; intros.
+  all: try(reflexivity || inversion H1).
+  all: try(destruct l); try(destruct l0); try(reflexivity || inversion H1).
+  * unfold eval, eval_arith. simpl. rewrite <- Z.add_comm. reflexivity.
+Qed.
+
+(*TODO: Not working*)
+(*
+Proposition plus_comm_extended {e1 e2 : ValueExpression} (v : ValueSequence + Exception) (eff eff2 : SideEffectList) : 
+  eval "+"%string [e1 ; e2] eff = (v, eff)
+->
+  exists v', eval "+"%string [e2; e1] eff2 = (v', eff2).
+Proof.
+  simpl. case_eq e1; case_eq e2; intros.
+  1-7, 9-36: eexists; try(inversion H1; reflexivity).
+  * eexists. reflexivity.
+Qed.
+*)
+
+Proposition plus_effect_unmodified {e1 e2 : ValueExpression} (v' : ValueSequence + Exception) (eff eff2 : SideEffectList) :
+  eval "+"%string [e1 ; e2] eff = (v', eff2)
+->
+  eff = eff2.
+Proof.
+  simpl. case_eq e1; case_eq e2; intros.
+  all: try(inversion H1; reflexivity).
+  all: try(destruct l); try(inversion H1; reflexivity).
+  all: destruct l0.
+Qed.
+
+Proposition plus_effect_changeable {v1 v2 : ValueExpression} (v' : ValueSequence + Exception) (eff eff2 : SideEffectList) :
+  eval "+"%string [v1; v2] eff = (v', eff)
+->
+  eval "+"%string [v1; v2] eff2 = (v', eff2).
+Proof.
+  intros. simpl in *. case_eq v1; case_eq v2; intros; subst.
+  all: try(inversion H; reflexivity).
+  all: try(destruct l); try(inversion H; reflexivity).
+  all: destruct l0; inversion H; auto.
+Qed.
+
+
+End Auxiliaries.
+
+(*TODO: Tests maybe for later. *)
+(*
+Section Tests.
+
+Import Auxiliaries.
+Import ListNotations.
+
+(** Tests *)
+
+Goal (eval "+" [VLit (Integer 1); VLit (Integer 2)]) [] = (inl [VLit (Integer 3)], []).
+Proof. reflexivity. Qed.
+Goal (eval "-" [VLit (Integer 1); VLit (Integer 2)]) [] = (inl [VLit (Integer (-1))], []).
+Proof. reflexivity. Qed.
+Goal (eval "+" [VLit (Atom "foo"); VLit (Integer 2)]) [] 
+    = (inr (badarith (VTuple [VLit (Atom "+"); VLit (Atom "foo"); VLit (Integer 2)])), []).
+Proof. reflexivity. Qed.
+Goal (eval "+" [VLit (Integer 1); VLit (Atom "foo")]) [] 
+    = (inr (badarith (VTuple [VLit (Atom "+"); VLit (Integer 1); VLit (Atom "foo")])), []).
+Proof. reflexivity. Qed.
+Goal (eval "-" [VLit (Atom "foo"); VLit (Integer 2)]) [] 
+    = (inr (badarith (VTuple [VLit (Atom "-"); VLit (Atom "foo"); VLit (Integer 2)])), []).
+Proof. reflexivity. Qed.
+Goal (eval "-" [VLit (Integer 1); VLit (Atom "foo")]) [] 
+    = (inr (badarith (VTuple [VLit (Atom "-"); VLit (Integer 1); VLit (Atom "foo")])), []).
+Proof. reflexivity. Qed.
+Goal (eval "-" [VLit (Atom "foo")]) [] 
+    = (inr (badarith (VTuple [VLit (Atom "-"); VLit (Atom "foo")])), []).
+Proof. reflexivity. Qed.
+Goal (eval "+" [VLit (Atom "foo")]) [] 
+    = (inr (badarith (VTuple [VLit (Atom "+"); VLit (Atom "foo")])), []).
+Proof. unfold eval, eval_arith. simpl. reflexivity. Qed.
+
+Goal (eval "bsl" [VLit (Integer 10); VLit (Integer 20)]) [] = (inl [VLit (Integer 10485760)], []).
+Proof. reflexivity. Qed.
+Goal (eval "bsr" [VLit (Integer 10); VLit (Integer 20)]) [] = (inl [VLit (Integer 0)], []).
+Proof. reflexivity. Qed.
+Goal (eval "bsl" [VLit (Atom "foo"); VLit (Integer 2)]) [] 
+    = (inr (badarith (VTuple [VLit (Atom "bsl"); VLit (Atom "foo"); VLit (Integer 2)])), []).
+Proof. reflexivity. Qed.
+Goal (eval "bsl" [VLit (Integer 1); VLit (Atom "foo")]) [] 
+    = (inr (badarith (VTuple [VLit (Atom "bsl"); VLit (Integer 1); VLit (Atom "foo")])), []).
+Proof. reflexivity. Qed.
+Goal (eval "bsr" [VLit (Atom "foo"); VLit (Integer 2)]) [] 
+    = (inr (badarith (VTuple [VLit (Atom "bsr"); VLit (Atom "foo"); VLit (Integer 2)])), []).
+Proof. reflexivity. Qed.
+Goal (eval "bsr" [VLit (Integer 1); VLit (Atom "foo")]) [] 
+    = (inr (badarith (VTuple [VLit (Atom "bsr"); VLit (Integer 1); VLit (Atom "foo")])), []).
+Proof. reflexivity. Qed.
+Goal (eval "bsl" [VLit (Atom "foo")]) [] 
+    = (inr (undef (VLit (Atom "bsl"))), []).
+Proof. unfold eval, eval_arith. simpl. reflexivity. Qed.
+Goal (eval "bsr" [VLit (Atom "foo")]) [] 
+    = (inr (undef (VLit (Atom "bsr"))), []).
+Proof. unfold eval, eval_arith. simpl. reflexivity. Qed.
+
+Goal (eval "not" [ttrue]) [] = (inl [ffalse], []). Proof. reflexivity. Qed.
+Goal (eval "not" [ffalse]) [] = (inl [ttrue], []). Proof. reflexivity. Qed.
+Goal (eval "not" [VLit (Integer 5)]) [] = (inr (badarg (VTuple [VLit (Atom "not"); VLit (Integer 5)])), []).
+Proof. reflexivity. Qed.
+Goal (eval "not" [VLit (Integer 5); VEmptyTuple]) [] = (inr (undef (VLit (Atom "not"))), []).
+Proof. reflexivity. Qed.
+
+Goal (eval "and" [ttrue; ttrue]) [] = (inl [ttrue], []). Proof. reflexivity. Qed.
+Goal (eval "and" [ttrue; ffalse]) [] = (inl [ffalse], []). Proof. reflexivity. Qed.
+Goal (eval "and" [ffalse; ttrue]) [] = (inl [ffalse], []). Proof. reflexivity. Qed.
+Goal (eval "and" [ffalse; ffalse]) [] = (inl [ffalse], []). Proof. reflexivity. Qed.
+Goal (eval "and" [ttrue; VEmptyTuple]) [] = (inr (badarg (VTuple [VLit (Atom "and"); ttrue; VTuple []])), []).
+Proof. reflexivity. Qed.
+Goal (eval "and" [ttrue]) [] = (inr (undef (VLit (Atom "and"))), []). Proof. reflexivity. Qed.
+
+Goal (eval "or" [ttrue; ttrue]) [] = (inl [ttrue], []). Proof. reflexivity. Qed.
+Goal (eval "or" [ttrue; ffalse]) [] = (inl [ttrue], []). Proof. reflexivity. Qed.
+Goal (eval "or" [ffalse; ttrue]) [] = (inl [ttrue], []). Proof. reflexivity. Qed.
+Goal (eval "or" [ffalse; ffalse]) [] = (inl [ffalse], []). Proof. reflexivity. Qed.
+Goal (eval "or" [ttrue; VEmptyTuple]) [] = (inr (badarg (VTuple [VLit (Atom "or"); ttrue; VTuple []])), []).
+Proof. reflexivity. Qed.
+Goal (eval "or" [ttrue]) [] = (inr (undef (VLit (Atom "or"))), []).
+Proof. reflexivity. Qed.
+
+Goal (eval "fwrite" [ttrue]) [] = (inl [ok], [(Output, [ttrue])]).
+Proof. reflexivity. Qed.
+Goal (eval "fwrite" [VMap [(ttrue, ttrue)]]) [] = (inl [ok], [(Output, [VMap [(ttrue, ttrue)]])]).
+Proof. reflexivity. Qed.
+Goal (eval "fwrite" []) [] = (inr (undef (VLit (Atom "fwrite"))), []).
+Proof. reflexivity. Qed.
+
+Goal (eval "fread" [VLit (Atom "foo.txt"); ttrue]) [] = 
+   (inl [VTuple [ok; ttrue]], [(Input, [VLit (Atom "foo.txt"); ttrue])]).
+Proof. reflexivity. Qed.
+Goal (eval "fread" [VLit (Atom "foo.txt"); VMap [(ttrue, ttrue)]]) [] = 
+   (inl [VTuple [ok; VMap [(ttrue, ttrue)]]], [(Input, [VLit (Atom "foo.txt"); VMap [(ttrue, ttrue)]])]).
+Proof. reflexivity. Qed.
+Goal (eval "fread" []) [] = (inr (undef (VLit (Atom "fread"))), []).
+Proof. reflexivity. Qed.
+
+Goal (eval "==" [ttrue; ttrue]) [] = (inl [ttrue], []).
+Proof. reflexivity. Qed.
+Goal (eval "==" [ttrue; ffalse]) [] = (inl [ffalse], []).
+Proof. reflexivity. Qed.
+Goal (eval "==" [VClos [] [] 1 [] EEmptyMap; ttrue]) [] = (inl [ffalse], []).
+Proof. reflexivity. Qed.
+Goal (eval "==" [VClos [] [] 1 [] EEmptyMap; VClos [] [] 2 [] EEmptyMap]) [] = (inl [ffalse], []).
+Proof. reflexivity. Qed.
+Goal (eval "==" [VClos [] [] 1 [] EEmptyMap; VClos [] [] 1 [] EEmptyMap]) [] = (inl [ttrue], []).
+Proof. reflexivity. Qed.
+
+Goal (eval "/=" [ttrue; ttrue]) [] = (inl [ffalse], []).
+Proof. reflexivity. Qed.
+Goal (eval "/=" [ttrue; ffalse]) [] = (inl [ttrue], []).
+Proof. reflexivity. Qed.
+Goal (eval "/=" [VClos [] [] 1 [] EEmptyMap; ttrue]) [] = (inl [ttrue], []).
+Proof. reflexivity. Qed.
+Goal (eval "/=" [VClos [] [] 1 [] EEmptyMap; VClos [] [] 2 [] EEmptyMap]) [] = (inl [ttrue], []).
+Proof. reflexivity. Qed.
+Goal (eval "/=" [VClos [] [] 1 [] EEmptyMap; VClos [] [] 1 [] EEmptyMap]) [] = (inl [ffalse], []).
+Proof. reflexivity. Qed.
+Goal (eval "/=" [ttrue]) [] = (inr (undef (VLit (Atom "/="))), []).
+Proof. reflexivity. Qed.
+
+Definition l1 : Value := VCons ttrue VNil.
+Definition l2 : Value := VCons ttrue ttrue.
+Definition l3 : Value := VCons (VCons ttrue ttrue) ttrue.
+Definition l4 : Value := VCons ttrue (VCons ttrue (VCons ttrue VNil)).
+Definition l5 : Value := VCons ttrue (VCons ttrue ttrue).
+
+Goal (eval "++" [ttrue; ttrue]) [] = (inr (badarg (VTuple [VLit (Atom "++"); ttrue; ttrue])), []).
+Proof. reflexivity. Qed.
+Goal (eval "++" [l1; l1]) [] = (inl [VCons ttrue (VCons ttrue VNil)], []).
+Proof. reflexivity. Qed.
+Goal (eval "++" [l1; l2]) [] = 
+  (inl [VCons ttrue (VCons ttrue ttrue)], []).
+Proof. reflexivity. Qed.
+Goal (eval "++" [l1; l3]) [] = 
+  (inl [VCons ttrue (VCons (VCons ttrue ttrue) ttrue)], []).
+Proof. reflexivity. Qed.
+Goal (eval "++" [l3; l3]) [] = 
+  (inr (badarg (VTuple [VLit (Atom "++"); VCons (VCons ttrue ttrue) ttrue; VCons (VCons ttrue ttrue) ttrue])), []).
+Proof.  unfold eval, eval_transform_list. simpl. reflexivity. Qed.
+Goal (eval "++" [l1; ErrorValue]) [] = (inl [VCons ttrue ErrorValue], []).
+Proof. unfold eval, eval_transform_list. simpl. reflexivity. Qed.
+
+Goal (eval "--" [ttrue; ttrue]) [] = (inr (badarg (VTuple [VLit (Atom "--"); ttrue; ttrue])), []).
+Proof. reflexivity. Qed.
+Goal (eval "--" [l1; l1]) [] = (inl [VNil], []).
+Proof. reflexivity. Qed.
+Goal (eval "--" [l1; l2]) [] = 
+  (inr (badarg (VTuple [VLit (Atom "--"); VCons ttrue VNil; VCons ttrue ttrue])), []).
+Proof. unfold eval, eval_transform_list. simpl. reflexivity. Qed.
+Goal (eval "--" [l1; l3]) [] = 
+  (inr (badarg (VTuple [VLit (Atom "--"); VCons ttrue VNil; VCons (VCons ttrue ttrue) ttrue])), []).
+Proof. reflexivity. Qed.
+Goal (eval "--" [l3; l3]) [] = 
+  (inr (badarg (VTuple [VLit (Atom "--"); VCons (VCons ttrue ttrue) ttrue;
+                        VCons (VCons ttrue ttrue) ttrue])), []).
+Proof. reflexivity. Qed.
+Goal (eval "--" [l3; l1]) [] =
+  (inr (badarg (VTuple [VLit (Atom "--"); VCons (VCons ttrue ttrue) ttrue; VCons ttrue VNil])), []).
+Proof. reflexivity. Qed.
+Goal (eval "--" [l4; l4]) [] = (inl [VNil], []).
+Proof. reflexivity. Qed.
+Goal (eval "--" [VCons (VLit (Integer 0)) (VCons (VLit (Atom "HIGH")) (VCons ffalse (VCons (VLit (Atom "FERTILE")) (VCons VNil VNil))));
+  VCons VNil (VCons (VLit (Integer 0)) VNil)
+] [])
+=
+  (inl [(VCons (VLit (Atom "HIGH")) (VCons ffalse (VCons (VLit (Atom "FERTILE")) VNil)))], []).
+Proof. unfold eval, eval_transform_list, eval_subtract. simpl. reflexivity. Qed.
+
+Goal (eval "tuple_to_list" [VTuple [ttrue; ttrue; ttrue; l1]] []) =
+  (inl [VCons ttrue (VCons ttrue (VCons ttrue (VCons (VCons ttrue VNil) VNil)))], []).
+Proof. reflexivity. Qed.
+Goal (eval "tuple_to_list" [VTuple [ttrue; ttrue; l5; l1]] []) =
+  (inl [VCons ttrue (VCons ttrue (VCons (VCons ttrue (VCons ttrue ttrue)) 
+                                 (VCons (VCons ttrue VNil) VNil)))], []).
+Proof. reflexivity. Qed.
+Goal (eval "tuple_to_list" [VTuple [ttrue; l3; ttrue; l1]] []) =
+  (inl [VCons ttrue (VCons (VCons (VCons ttrue ttrue) ttrue) (VCons ttrue (VCons (VCons ttrue VNil) VNil)))], []).
+Proof. reflexivity. Qed.
+Goal (eval "tuple_to_list" [VTuple [ttrue; ttrue; l2; l1]] []) =
+  (inl [VCons ttrue (VCons ttrue (VCons (VCons ttrue ttrue) (VCons (VCons ttrue VNil) VNil)))], []).
+Proof. reflexivity. Qed.
+Goal (eval "tuple_to_list" [ttrue] []) = 
+  (inr (badarg (VTuple [VLit (Atom "tuple_to_list"); ttrue])), []).
+Proof. reflexivity. Qed.
+
+Goal (eval "list_to_tuple" [l1] []) = (inl [VTuple [VLit (Atom "true")]], []).
+Proof. reflexivity. Qed.
+Goal (eval "list_to_tuple" [l2] []) =
+  (inr (badarg (VTuple [VLit (Atom "list_to_tuple"); VCons ttrue ttrue])), []).
+Proof. reflexivity. Qed.
+Goal (eval "list_to_tuple" [l3] []) =
+  (inr (badarg (VTuple [VLit (Atom "list_to_tuple"); VCons (VCons ttrue ttrue) ttrue])), []).
+Proof. reflexivity. Qed.
+Goal (eval "list_to_tuple" [l4] []) =
+  (inl [VTuple [VLit (Atom "true"); VLit (Atom "true"); VLit (Atom "true")]], []).
+Proof. reflexivity. Qed.
+Goal (eval "list_to_tuple" [l5] []) =
+  (inr (badarg (VTuple [VLit (Atom "list_to_tuple"); VCons ttrue ttrue])), []).
+Proof. reflexivity. Qed.
+
+Goal (eval "<" [ttrue; ttrue]) [] = (inl [ffalse], []).
+Proof. reflexivity. Qed.
+Goal (eval "<" [ttrue; ffalse]) [] = (inl [ffalse], []).
+Proof. reflexivity. Qed.
+Goal (eval "<" [VClos [] [] 1 [] EEmptyMap; VEmptyMap]) [] = (inl [ttrue], []).
+Proof. reflexivity. Qed.
+Goal (eval "<" [VClos [] [] 1 [] EEmptyMap; VClos [] [] 2 [] EEmptyMap]) [] = (inl [ttrue], []).
+Proof. reflexivity. Qed.
+Goal (eval "<" [VClos [] [] 1 [] EEmptyMap; VClos [] [] 1 [] EEmptyMap]) [] = (inl [ffalse], []).
+Proof. reflexivity. Qed.
+
+Goal (eval "=<" [ttrue; ttrue]) [] = (inl [ttrue], []).
+Proof. reflexivity. Qed.
+Goal (eval "=<" [ttrue; ffalse]) [] = (inl [ffalse], []).
+Proof. reflexivity. Qed.
+Goal (eval "=<" [VClos [] [] 1 [] EEmptyMap; VEmptyMap]) [] = (inl [ttrue], []).
+Proof. reflexivity. Qed.
+Goal (eval "=<" [VClos [] [] 1 [] EEmptyMap; VClos [] [] 2 [] EEmptyMap]) [] = (inl [ttrue], []).
+Proof. reflexivity. Qed.
+Goal (eval "=<" [VClos [] [] 1 [] EEmptyMap; VClos [] [] 1 [] EEmptyMap]) [] = (inl [ttrue], []).
+Proof. reflexivity. Qed.
+
+Goal (eval ">" [ttrue; ttrue]) [] = (inl [ffalse], []).
+Proof. reflexivity. Qed.
+Goal (eval ">" [ffalse; ttrue]) [] = (inl [ffalse], []).
+Proof. reflexivity. Qed.
+Goal (eval ">" [VEmptyMap; VClos [] [] 1 [] EEmptyMap]) [] = (inl [ttrue], []).
+Proof. reflexivity. Qed.
+Goal (eval ">" [VClos [] [] 2 [] EEmptyMap; VClos [] [] 1 [] EEmptyMap]) [] = (inl [ttrue], []).
+Proof. reflexivity. Qed.
+Goal (eval ">" [VClos [] [] 1 [] EEmptyMap; VClos [] [] 1 [] EEmptyMap]) [] = (inl [ffalse], []).
+Proof. reflexivity. Qed.
+
+Goal (eval ">=" [ttrue; ttrue]) [] = (inl [ttrue], []).
+Proof. reflexivity. Qed.
+Goal (eval ">=" [ffalse; ttrue]) [] = (inl [ffalse], []).
+Proof. reflexivity. Qed.
+Goal (eval ">=" [VEmptyMap; VClos [] [] 1 [] EEmptyMap]) [] = (inl [ttrue], []).
+Proof. reflexivity. Qed.
+Goal (eval ">=" [VClos [] [] 2 [] EEmptyMap; VClos [] [] 1 [] EEmptyMap]) [] = (inl [ttrue], []).
+Proof. reflexivity. Qed.
+Goal (eval ">=" [VClos [] [] 1 [] EEmptyMap; VClos [] [] 1 [] EEmptyMap]) [] = (inl [ttrue], []).
+Proof. reflexivity. Qed.
+
+Goal (eval "length" [l1]) [] = (inl [VLit (Integer 1)], []).
+Proof. reflexivity. Qed.
+Goal (eval "length" [l2]) [] = (inr (badarg (VTuple [VLit (Atom "length");l2])), []).
+Proof. reflexivity. Qed.
+Goal (eval "length" [l3]) [] = (inr (badarg (VTuple [VLit (Atom "length");l3])), []).
+Proof. reflexivity. Qed.
+Goal (eval "length" [l4]) [] = (inl [VLit (Integer 3)], []).
+Proof. reflexivity. Qed.
+Goal (eval "length" [l5]) [] = (inr (badarg (VTuple [VLit (Atom "length");l5])), []).
+Proof. reflexivity. Qed.
+Goal (eval "length" [ttrue]) [] = (inr (badarg (VTuple [VLit (Atom "length");ttrue])), []).
+Proof. reflexivity. Qed.
+Goal (eval "length" [l5;l3]) [] = (inr (undef (VLit (Atom "length"))), []).
+Proof. reflexivity. Qed.
+
+Goal (eval "tuple_size" [l3]) [] = (inr (badarg (VTuple [VLit (Atom "tuple_size");l3])), []).
+Proof. reflexivity. Qed.
+Goal (eval "tuple_size" [VTuple []]) [] = (inl [VLit (Integer 0)], []).
+Proof. reflexivity. Qed.
+Goal (eval "tuple_size" [VTuple [ttrue;ttrue;ttrue]]) [] = (inl [VLit (Integer 3)], []).
+Proof. reflexivity. Qed.
+Goal (eval "tuple_size" [VTuple [ttrue;ttrue;ttrue]; ErrorValue]) [] = (inr (undef (VLit (Atom "tuple_size"))), []).
+Proof. reflexivity. Qed.
+
+
+Goal (eval "hd" [l1]) [] = (inl [ttrue], []).
+Proof. reflexivity. Qed.
+Goal (eval "hd" [VNil]) [] = (inr (badarg (VTuple [VLit (Atom "hd");VNil])), []).
+Proof. reflexivity. Qed.
+Goal (eval "hd" [l2]) [] = (inl [ttrue], []).
+Proof. reflexivity. Qed.
+Goal (eval "hd" [l3]) [] = (inl [(VCons ttrue ttrue)], []).
+Proof. reflexivity. Qed.
+Goal (eval "hd" [l4]) [] = (inl [ttrue], []).
+Proof. reflexivity. Qed.
+Goal (eval "hd" [l5]) [] = (inl [ttrue], []).
+Proof. unfold l5. reflexivity. Qed.
+Goal (eval "hd" [ttrue]) [] = (inr (badarg (VTuple [VLit (Atom "hd");ttrue])), []).
+Proof. reflexivity. Qed.
+Goal (eval "hd" [l5;l3]) [] = (inr (undef (VLit (Atom "hd"))), []).
+Proof. reflexivity. Qed.
+
+Goal (eval "tl" [l1]) [] = (inl [VNil], []).
+Proof. reflexivity. Qed.
+Goal (eval "tl" [VNil]) [] = (inr (badarg (VTuple [VLit (Atom "tl");VNil])), []).
+Proof. reflexivity. Qed.
+Goal (eval "tl" [l2]) [] = (inl [ttrue], []).
+Proof. reflexivity. Qed.
+Goal (eval "tl" [l3]) [] = (inl [ttrue], []).
+Proof. reflexivity. Qed.
+Goal (eval "tl" [l4]) [] = (inl [(VCons ttrue (VCons ttrue VNil))], []).
+Proof. reflexivity. Qed.
+Goal (eval "tl" [l5]) [] = (inl [VCons ttrue ttrue], []).
+Proof. unfold l5. reflexivity. Qed.
+Goal (eval "tl" [ttrue]) [] = (inr (badarg (VTuple [VLit (Atom "tl");ttrue])), []).
+Proof. reflexivity. Qed.
+Goal (eval "tl" [l5;l3]) [] = (inr (undef (VLit (Atom "tl"))), []).
+Proof. reflexivity. Qed.
+
+
+Goal (eval "element" [VLit (Integer 2); VTuple [ttrue]]) [] = (inr (badarg (VTuple [VLit (Atom "element"); VLit (Integer 2); VTuple [ttrue]])), []).
+Proof. unfold eval, eval_elem_tuple. simpl. reflexivity. Qed.
+Goal (eval "element" [VLit (Integer 1); VTuple [ttrue]]) [] = (inl [ttrue], []).
+Proof. reflexivity. Qed.
+Goal (eval "element" [ttrue; ttrue]) [] = (inr (badarg (VTuple [VLit (Atom "element"); ttrue; ttrue])), []).
+Proof. reflexivity. Qed.
+Goal (eval "element" [ttrue]) [] = (inr (undef (VLit (Atom "element"))), []).
+Proof. reflexivity. Qed.
+
+Goal (eval "setelement" [VLit (Integer 2); VTuple [ttrue]; ffalse]) [] = (inr (badarg (VTuple [VLit (Atom "setelement"); VLit (Integer 2); VTuple [ttrue]; ffalse])), []).
+Proof. unfold eval, eval_elem_tuple. simpl. reflexivity. Qed.
+Goal (eval "setelement" [VLit (Integer 1); VTuple [ttrue]; ffalse]) [] = (inl [VTuple [ffalse]], []).
+Proof. reflexivity. Qed.
+Goal (eval "setelement" [ttrue; ttrue; ttrue]) [] = (inr (badarg (VTuple [VLit (Atom "setelement"); ttrue; ttrue; ttrue])), []).
+Proof. unfold eval, eval_elem_tuple. simpl. reflexivity. Qed.
+Goal (eval "setelement" [ttrue]) [] = (inr (undef (VLit (Atom "setelement"))), []).
+Proof. reflexivity. Qed.
+
+Goal eval "is_number" [VLit (Integer 2)] [] = (inl [ttrue], []).
+Proof. reflexivity. Qed.
+Goal eval "is_number" [ffalse] [] = (inl [ffalse], []).
+Proof. reflexivity. Qed.
+Goal eval "is_number" [ffalse; ffalse] [] = (inr (undef (VLit (Atom "is_number"))), []).
+Proof. reflexivity. Qed.
+Goal eval "is_integer" [VLit (Integer 2)] [] = (inl [ttrue], []).
+Proof. reflexivity. Qed.
+Goal eval "is_integer" [ffalse] [] = (inl [ffalse], []).
+Proof. reflexivity. Qed.
+Goal eval "is_integer" [ffalse; ffalse] [] = (inr (undef (VLit (Atom "is_integer"))), []).
+Proof. reflexivity. Qed.
+Goal eval "is_atom" [VLit (Integer 2)] [] = (inl [ffalse], []).
+Proof. reflexivity. Qed.
+Goal eval "is_atom" [VLit (Atom "foo")] [] = (inl [ttrue], []).
+Proof. reflexivity. Qed.
+Goal eval "is_atom" [ffalse; ffalse] [] = (inr (undef (VLit (Atom "is_atom"))), []).
+Proof. reflexivity. Qed.
+Goal eval "is_boolean" [VLit (Integer 2)] [] = (inl [ffalse], []).
+Proof. reflexivity. Qed.
+Goal eval "is_boolean" [ttrue] [] = (inl [ttrue], []).
+Proof. reflexivity. Qed.
+Goal eval "is_boolean" [ffalse] [] = (inl [ttrue], []).
+Proof. reflexivity. Qed.
+Goal eval "is_boolean" [ffalse; ffalse] [] = (inr (undef (VLit (Atom "is_boolean"))), []).
+Proof. reflexivity. Qed.
+
+Goal eval "error" [ffalse; ffalse] [] = (inr (Error, ffalse, ffalse), []).
+Proof. reflexivity. Qed.
+Goal eval "error" [ffalse] [] = (inr (Error, ffalse, VNil), []).
+Proof. reflexivity. Qed.
+Goal eval "error" [] [] = (inr (undef ErrorValue), []).
+Proof. reflexivity. Qed.
+
+
+End Tests.
+*)
